Minor adjustments; (partially) filled some holes. Isolated proof that CompilerCorrect implies fwd_sim in extra file.

veric/sim.v
@@ -609,51 +609,8 @@ Lemma val_listless_forall_lessdef: forall args args' (H:Val.lessdef_list args ar
     induction args; intros;  inv H; constructor; eauto.
   Qed. 
 
-Require Import compcert.Smallstep.
-Section CoreSem_to_semantics.
-    Variables (F C V:Type).
-    Let genv  := Genv.t F V.
-    Variable (Sem:CompcertCoreSem genv C (list (ident * globvar V))). (*HERE we specialize type D to program variables*)
-
-    Let state := (C * mem)%type.
-
-    Inductive step (ge:genv) : state -> trace -> state -> Prop :=
-    | step_corestep : forall c m c' m',
-          corestep Sem ge c m c' m' ->
-          step ge (c,m) E0 (c',m')
-
-    | step_ext_step : forall c m c' m' ef args tr ret,
-          at_external Sem c = Some (ef,args) ->
-          external_call ef ge args m tr ret m' ->
-          after_external Sem ret c = Some c' ->
-          step ge (c,m) tr (c',m').
-
-    Variable (prog:AST.program F V).
-
-    (*Definition main_sig : signature := 
-       mksignature (AST.Tint :: AST.Tint :: nil) (Some AST.Tint).*)
-    Definition main_sig : signature := 
-       mksignature (nil) (Some AST.Tint).
-
-    Definition initial_state (st:state) : Prop :=
-      exists b, exists vals,
-        Forall2 (val_inject (Mem.flat_inj (Mem.nextblock (snd st)))) vals vals /\
-        Forall2 Val.has_type vals (sig_args main_sig) /\
-        Genv.find_symbol (Genv.globalenv prog) (prog_main prog) = Some b /\
-        make_initial_core Sem (Genv.globalenv prog) (Vptr b Int.zero) vals = Some (fst st) /\
-        Genv.init_mem prog = Some (snd st). 
-
-    Definition final_state (st:state) (i:int) : Prop :=
-      safely_halted Sem (Genv.globalenv prog) (fst st) = Some i.
-
-   Definition mk_semantics: semantics :=
-           Semantics  step initial_state final_state (Genv.globalenv prog).
-
-End CoreSem_to_semantics.
-Check mk_semantics. 
 
 Module CompilerCorrectness.
-
 Definition globvar_eq {V1 V2: Type} (v1:globvar V1) (v2:globvar V2) :=
     match v1, v2 with mkglobvar _ init1 readonly1 volatile1, mkglobvar _ init2 readonly2 volatile2 =>
                         init1 = init2 /\ readonly1 =  readonly2 /\ volatile1 = volatile2
@@ -697,13 +654,11 @@ Definition externvars_ok  {F1 V1:Type}  (P1 : AST.program F1 V1)
          forall b v, Genv.find_var_info  (Genv.globalenv P1) b = Some v -> 
                         exists e, Genv.find_symbol (Genv.globalenv P1) e = Some b /\ In (e,extern_globvar) ExternIdents.
 
-Definition GenvHyp {F1 V1 C1 F2 V2 C2} 
-               (Sem1 : CompcertCoreSem (Genv.t F1 V1) C1 (list (ident * globvar V1)))
-               (Sem2 : CompcertCoreSem (Genv.t F2 V2) C2 (list (ident * globvar V2)))
+Definition GenvHyp {F1 V1 F2 V2} 
                (P1 : AST.program F1 V1) (P2 : AST.program F2 V2): Prop :=
        (forall id : ident,
-                                 Genv.find_symbol (globalenv (mk_semantics F2 C2 V2 Sem2 P2)) id =
-                                 Genv.find_symbol (globalenv (mk_semantics F1 C1 V1 Sem1 P1)) id)
+                                 Genv.find_symbol (Genv.globalenv P2) id =
+                                 Genv.find_symbol (Genv.globalenv P1) id)
        /\ (forall b : block,
                                           block_is_volatile (Genv.globalenv P2) b =
                                           block_is_volatile (Genv.globalenv P1) b).
@@ -730,7 +685,7 @@ Inductive compiler_correctness (I: forall F C V  (Sem : CompcertCoreSem (Genv.t 
                prog_main P1 = prog_main P2 -> 
 
 (*HERE IS THE INJECTION OF THE GENV-ASSUMPTIONS INTO THE PROOF:*)
-               GenvHyp Sem1 Sem2 P1 P2 ->
+               GenvHyp P1 P2 ->
 
                 I _ _ _  Sem1 P1 -> I _ _ _  Sem2 P2 -> 
                compiler_correctness I ExternIdents F1 C1 V1 F2 C2 V2 Sem1 Sem2 P1 P2
@@ -749,7 +704,7 @@ Inductive compiler_correctness (I: forall F C V  (Sem : CompcertCoreSem (Genv.t 
                prog_main P1 = prog_main P2 -> 
 
                (*HERE IS THE INJECTION OF THE GENV-ASSUMPTIONS INTO THE PROOF:*)
-               GenvHyp Sem1 Sem2 P1 P2 ->
+               GenvHyp P1 P2 ->
 
                 I _ _ _ Sem1 P1 -> I _ _ _ Sem2 P2 -> 
                compiler_correctness I ExternIdents F1 C1 V1 F2 C2 V2 Sem1 Sem2 P1 P2
@@ -768,7 +723,7 @@ Inductive compiler_correctness (I: forall F C V  (Sem : CompcertCoreSem (Genv.t 
                prog_main P1 = prog_main P2 ->
 
                (*HERE IS THE INJECTION OF THE GENV-ASSUMPTIONS INTO THE PROOF:*)
-               GenvHyp Sem1 Sem2 P1 P2 ->
+               GenvHyp P1 P2 ->
                 externvars_ok P1 ExternIdents ->
 
                 I _ _ _ Sem1 P1 -> I _ _ _ Sem2 P2 -> 
@@ -809,330 +764,11 @@ Lemma cc_Genv:forall {F1 C1 V1 F2 C2 V2}
                (P1 : AST.program F1 V1)
                (P2 : AST.program F2 V2)  ExternIdents I,
                     compiler_correctness I ExternIdents F1 C1 V1 F2 C2 V2 Sem1 Sem2 P1 P2 ->
-               GenvHyp Sem1 Sem2 P1 P2.
+               GenvHyp P1 P2.
    Proof. intros. induction X; intuition. 
        destruct IHX1.
        destruct IHX2.
         split; intros; eauto. rewrite H1. apply H. Qed.
 End CompilerCorrectness.
 
-Module COMPILER_CORRECTNESS_COMPCERT_SIM.
-
-  Lemma corestep_plus_step: forall F C V (Sem:CompcertCoreSem (Genv.t F V) C  (list (ident * globvar V))) P c m c' m',
-         corestep Sem (Genv.globalenv P) c m c' m' ->
-         plus (step F C V Sem) (Genv.globalenv P) (c, m) E0 (c', m').
-    Proof. intros.  eapply plus_left. eapply step_corestep. apply H.  apply star_refl. rewrite E0_left. trivial. Qed.
-
-  Lemma corestep_plus_plus_step: forall F C V (Sem:CompcertCoreSem (Genv.t F V) C (list (ident * globvar V))) P c m c' m',
-              corestep_plus Sem (Genv.globalenv P) c m c' m' -> plus (step F C V Sem) (Genv.globalenv P) (c, m) E0 (c', m').
-    Proof. intros. unfold corestep_plus in H. destruct H as [n Hn].
-       generalize dependent m.  generalize dependent c. 
-      induction n.
-         simpl; intros. destruct Hn as [c2 [m2 [Hstep X]]]. inv X. eapply corestep_plus_step; auto.
-      intros. simpl in Hn. destruct Hn as [c1 [m1 [Hstep X]]].
-          eapply plus_left. eapply step_corestep. apply Hstep.
-             eapply plus_star. eapply IHn. apply X.  rewrite E0_left. trivial.
-   Qed.
-
-  Lemma corestep_star_star_step: forall F C V (Sem:CompcertCoreSem (Genv.t F V) C  (list (ident * globvar V))) P c m c' m',
-              corestep_star Sem (Genv.globalenv P) c m c' m' -> star (step F C V Sem) (Genv.globalenv P) (c, m) E0 (c', m').
-    Proof. intros. unfold corestep_star in H. destruct H as [n Hn].
-      destruct n; simpl in Hn. inv Hn. apply star_refl. 
-      eapply plus_star. eapply corestep_plus_plus_step. exists n. apply Hn.
-    Qed.
-
-(*LENB: MAYBE INSTEAD OF USING THIS (INCORRECT) LEMMA IN THE PROOF BELOW
-WE CAN SOMEHOW ADD A HYPOTHESIS meminj_preserves_globals ge j
-SOMEWHERE IN cc_inj OR Sim_inj.at_external or Sim_inj.after_external?
-CURRENTLY WE DON'T HAVE THE ge aAVILABLE THERE...*)
-Lemma meminj_preserves_globals_inject_incr: forall {F V} (ge: Genv.t F V) j j'
-              (MPj: meminj_preserves_globals ge j) (InjJ : inject_incr j j'),
-              meminj_preserves_globals ge j'.
-  Proof. intros.
-       destruct MPj as [MP1 [MP2 MP3]].
-       split. clear MP2 MP3. intros. apply InjJ. eapply MP1. apply H.
-       split. clear MP1 MP3. intros. apply InjJ. eapply MP2. apply H.
-       intros. admit. (*does not hold*)
-  Qed.
-
-Theorem CompilerCorrectness_implies_CompcertForwardSimulation:
-     forall F1 C1 V1 F2 C2 V2
-        (Sem1: CompcertCoreSem (Genv.t F1 V1) C1 (list (ident * globvar V1)))
-        (Sem2: CompcertCoreSem (Genv.t F2 V2) C2  (list (ident * globvar V2)))
-        P1 P2 ExternIdents,
-        In (P1.(prog_main), CompilerCorrectness.extern_func main_sig) ExternIdents  -> P1.(prog_main) = P2.(prog_main) ->
-        CompilerCorrectness.compiler_correctness
-             (fun F C V Sem P => (forall x, Genv.init_mem P = Some x <-> initial_mem Sem (Genv.globalenv P) x P.(prog_vars)))
-              ExternIdents F1 C1 V1 F2 C2 V2 Sem1 Sem2 P1 P2 ->
-        forward_simulation (mk_semantics F1 C1 V1 Sem1 P1)  (mk_semantics F2 C2 V2 Sem2 P2).
-Proof.
-  intros.
-  induction X; intros.
-  Focus 4. (*trans_case*)
-     assert (MM: prog_main P1 = prog_main P2). eapply CompilerCorrectness.cc_main; eauto.
-      spec IHX1.  apply H.
-      spec IHX1. apply MM.  
-      spec IHX2. rewrite MM in H. apply H.
-      spec IHX2. eapply CompilerCorrectness.cc_main; eauto.
-      clear X1 X2.
-      eapply compose_forward_simulation; eauto.
-  (*equals_case*)
-        rename i into GenvInit1; rename i0 into GenvInit2.
-        destruct g as [HypGenv HypVolatile].
-        set (fsim_index := Sim_eq.core_data R).
-        set (fsim_order := Sim_eq.core_ord R).
-        set (fsim_order_wf := Sim_eq.core_ord_wf R).
-        set (fsim_match_states s (x:C1 * mem) (y:C2 * mem) :=
-                          Sim_eq.match_core R s (fst x) (fst y) /\ snd x = snd y).
-        apply ( @Forward_simulation  (mk_semantics F1 C1 V1 Sem1 P1)  (mk_semantics F2 C2 V2 Sem2 P2)
-                        fsim_index fsim_order fsim_order_wf  fsim_match_states).
-             (*initial_state*) simpl. unfold initial_state. intros.
-                      destruct s1 as [c1 m1].
-                      destruct H1 as [b [args [K1 [ K2 [K3 [K4 K5]]]]]].
-                      destruct (ePts_ok _ _ H) as [bb [KK1 [KK2 [KK3 KK4]]]].
-                      assert (X := @Sim_eq.core_initial _ _ _ _ _ _ Sem1 Sem2  (Genv.globalenv P1) (Genv.globalenv P2)  entrypoints R _ _ _ KK3 nil).
-                      simpl in X.  destruct X. constructor. 
-                            destruct H1 as [cc1 [cc2 [ini1 [ini2 mtch]]]].
-                          exists x. exists (cc2,m1).
-                         split. simpl. exists bb. exists nil. simpl.
-                             repeat  split; try constructor. rewrite <- H0. apply KK2.
-                                assumption.
-                           destruct (Eq_init m1).  apply GenvInit1. apply K5. destruct H1; subst. simpl in *. apply GenvInit2. apply H1. 
-                      simpl. hnf. simpl in *. split; trivial. rewrite K3 in KK1. inv KK1.  inv K2. rewrite K4 in ini1.  inv ini1. assumption.
-           (*finalstate*)
-                 clear GenvInit1 GenvInit2.
-                 simpl. unfold final_state. intros. destruct s1 as [c1 m1]. destruct s2 as [c2 m2]. simpl in *.
-                      destruct H1. simpl in H3. subst.  simpl in *.
-                      apply (Sim_eq.core_halted R _ _ _ _ H1 H2).
-                      (*apply (@Sim_eq.core_halted _ _ _ _ Sem1 Sem2 (Genv.globalenv P1) (Genv.globalenv P2)  entrypoints R _ _ _ _ H1 H2).*)
-           (*diagram*)
-                 clear GenvInit1 GenvInit2.
-                 simpl. subst fsim_match_states. simpl. intros.
-                destruct s1 as [c1 m1]. destruct s2 as [c2 m2].  destruct s1' as [c1' m1'].  simpl in *.
-                      destruct H2. subst.
-                 inv H1.
-                 (*corestep*)  
-                   assert (DD := @Sim_eq.core_diagram _ _ _ _ _ _ Sem1 Sem2 (Genv.globalenv P1) (Genv.globalenv P2) entrypoints R _ _ _ _ H6 _ _ H2).
-                   destruct DD as [c2' [d' [MC myStep]]].
-                  exists d'. exists (c2', m1'); simpl. split; auto.
-                    destruct myStep.
-                      (*case corestep_plus*) left. eapply corestep_plus_plus_step; eauto.
-                      (*case core_step_star*) right.  destruct H1. split; auto. apply corestep_star_star_step; eauto.
-               (*external_step*) 
-                    destruct (@Sim_eq.core_at_external _ _ _ _ _ _ Sem1 Sem2 (Genv.globalenv P1) (Genv.globalenv P2) entrypoints R _ _ _ _ _ H2 H8) as [AtExt2 TP].
-                    assert (DD := @Sim_eq.core_after_external _ _ _ _ _ _ Sem1 Sem2 (Genv.globalenv P1) (Genv.globalenv P2) entrypoints R).
-                    assert (RetTp:= external_call_well_typed _ _ _ _ _ _ _ H9).
-                    destruct (DD _ _ _ ret _ _ H2 H8 AtExt2 TP RetTp) as [c1'' [c2' [d' [AftExt1 [AftExt2 CM]]]]]; clear DD.
-                    rewrite AftExt1 in H10. inv H10.
-                    exists d'. exists (c2', m1'). simpl.
-                    split; auto. left.  eapply plus_one. eapply step_ext_step. apply AtExt2. Focus 2. apply AftExt2.
-                                 apply external_call_symbols_preserved_gen with (ge1:=(Genv.globalenv P1)).
-                                        apply HypGenv. (*HERE*)
-                                        apply HypVolatile. (*HERE*)
-                                        apply H9. 
-         (* fsim_symbols_preserved*) simpl. apply HypGenv. (*SAME HERE*) 
-   (*extends*) 
-        rename i into GenvInit1; rename i0 into GenvInit2.
-        destruct g as [HypGenv HypVolatile].
-        set (fsim_index := Sim_ext.core_data R).
-        set (fsim_order := Sim_ext.core_ord R).
-        set (fsim_order_wf := Sim_ext.core_ord_wf R).
-        set (fsim_match_states s (x:C1 * mem) (y:C2 * mem) :=
-                        Sim_ext.match_state R s (fst x)  (snd x) (fst y) (snd y)).
-        apply ( @Forward_simulation  (mk_semantics F1 C1 V1 Sem1 P1)  (mk_semantics F2 C2 V2 Sem2 P2)
-                        fsim_index fsim_order fsim_order_wf  fsim_match_states).
-             (*initial_state*) simpl. unfold initial_state. intros.
-                      destruct s1 as [c1 m1]. simpl in *.
-                      destruct H1 as [b [args [K1 [ K2 [K3 [K4 K5]]]]]].
-                       destruct (ePts_ok _ _ H) as [b1 [KK1 [KK2 [Hfound [f1 [f2 [Hf1 Hf2]]]]]]].
-                       rewrite KK1 in K3. inv K3. inv K2. clear K1 ePts_ok H.
-                       apply GenvInit1 in K5. apply Extends_init in K5. destruct K5 as [m2 [iniMem2 Mextends]].
-                      assert (X := @Sim_ext.core_initial _ _ _ _ _ _ Sem1 Sem2  (Genv.globalenv P1) (Genv.globalenv P2)  entrypoints R _ _ _ Hfound nil nil m1 m2).
-                      destruct X as [d' [c1' [c2' [IniCore1 [IniCore2 ExtMatch]]]]].
-                          constructor.
-                          constructor.
-                          assumption.
-                    rewrite IniCore1 in K4. inv K4.
-                    exists d'. exists (c2', m2); simpl. 
-                         split; auto. 
-                          exists b. exists nil. simpl.
-                          repeat  split; try constructor. 
-                          rewrite <- H0. apply KK2.  
-                         assumption.
-                         apply GenvInit2. apply iniMem2. 
-           (*finalstate*)
-                 clear GenvInit1 GenvInit2.
-                 simpl. unfold final_state. intros. destruct s1 as [c1 m1]. destruct s2 as [c2 m2]. simpl in *.
-                    apply (Sim_ext.core_halted R _ _ _ _ _ _ H1 H2).
-                    (*apply (@Sim_ext.core_halted _ _ _ _ Sem1 Sem2  (Genv.globalenv P1) (Genv.globalenv P2)  entrypoints R _ _ _ _ _ _ H1 H2).*)
-           (*diagram*)
-                 clear GenvInit1 GenvInit2.
-                 simpl. subst fsim_match_states. simpl. intros.
-                destruct s1 as [c1 m1]. destruct s2 as [c2 m2].  destruct s1' as [c1' m1'].  simpl in *.
-                 inv H1. 
-                 (*corestep*)  
-                   assert (DD := @Sim_ext.core_diagram _ _ _ _ _ _ Sem1 Sem2 (Genv.globalenv P1) (Genv.globalenv P2) entrypoints R _ _ _ _ H6 _ _ _ H2).
-                   destruct DD as [c2' [m2' [d'  [MC' myStep]]]].
-                  exists d'. exists (c2', m2'); simpl. split; auto.
-                    destruct myStep.
-                      (*case corestep_plus*) left. eapply corestep_plus_plus_step; eauto.
-                      (*case core_step_star*) right.  destruct H1. split; auto. apply corestep_star_star_step; eauto.
-               (*external_step*) 
-                    destruct (@Sim_ext.core_at_external _ _ _ _ _ _ Sem1 Sem2 (Genv.globalenv P1) (Genv.globalenv P2) entrypoints R _ _ _ _ _ _ _ H2 H8) as [args2 [Mextends [lessArgs [TpArgs2 AtExt2]]]].
-                   assert (EXT:= @external_call_mem_extends _ _ _ _ _ _ _ _ _  _ _ H9 Mextends (forall_lessdef_val_listless _ _ lessArgs)).
-                   destruct EXT as [ret2 [m2' [extCall2 [lessRet [Mextends' MunchOn]]]]].
-                   assert (extCall2Genv2 : external_call ef (Genv.globalenv P2) args2 m2 t ret2 m2').
-                         eapply external_call_symbols_preserved_gen. 
-                             apply HypGenv. (*HERE*) 
-                             apply HypVolatile. (*HERE*)
-                             apply extCall2.
-                         (*An alternative would be to use this proof of extCall2Genv2:
-                                    apply (@external_call_symbols_preserved_2 ef F1 V1 F2 V2 (fun v1 =>Errors.Error nil)) with (ge1:=(Genv.globalenv P1)).
-                                          apply extCall2.
-                                          apply HypGenv. (*HERE*) 
-                                          simpl. intros.  assert (ECP:= external_call_spec ef). admit. (*first hyp on globvars*) 
-                                          simpl. admit. (*second hyp on globvars*) 
-                           *)
-                    clear extCall2.
-                    assert (DD := @Sim_ext.core_after_external _ _ _ _ _ _ Sem1 Sem2 (Genv.globalenv P1) (Genv.globalenv P2) entrypoints R _ _ _ _ _ _ _ _ ret ret2 m1' m2' H2 H8 AtExt2 lessArgs TpArgs2).
-                    destruct DD as [c1'' [c2' [d' [AftExt1 [AftExt2 Match']]]]].
-                            eapply external_call_mem_forward; eauto.
-                            eapply external_call_mem_forward; eauto.
-                            assumption.
-                            assumption.
-                            assumption.
-                            apply (external_call_well_typed _ _ _ _ _ _ _ extCall2Genv2). 
-                    rewrite AftExt1 in H10. inv H10.
-                      exists d'. exists (c2', m2'); simpl.
-                     split; auto. left.  eapply plus_one.
-                               apply step_ext_step with (ef:=ef)(args:=args2)(ret:=ret2).
-                                    apply AtExt2. 
-                                    apply extCall2Genv2.
-                                    assumption.
-         (* fsim_symbols_preserved*) simpl. apply HypGenv. (*SAME HERE*)  
-   (*inject*)
-        rename i into GenvInit1; rename i0 into GenvInit2.
-        destruct g as [HypGenv HypVolatile].
-        set (fsim_index := Sim_inj.core_data R).
-        set (fsim_order := Sim_inj.core_ord R).
-        set (fsim_order_wf := Sim_inj.core_ord_wf R).
-        set (fsim_match_states s (x:C1 * mem) (y:C2 * mem) :=
-                        exists j,  inject_incr jInit j /\  Sim_inj.match_state R s j (fst x)  (snd x) (fst y) (snd y)).
-        apply ( @Forward_simulation  (mk_semantics F1 C1 V1 Sem1 P1)  (mk_semantics F2 C2 V2 Sem2 P2)
-                        fsim_index fsim_order fsim_order_wf  fsim_match_states).
-             (*initial_state*) simpl. unfold initial_state. intros.
-                      destruct s1 as [c1 m1]. simpl in *.
-                      destruct H1 as [b [args [K1 [ K2 [K3 [K4 K5]]]]]].
-                       destruct (ePts_ok _ _ H) as [b1 [b2 [KK1 [KK2 [Hjb [Hfound [f1 [f2 [Hf1 Hf2]]]]]]]]].
-                      rewrite KK1 in K3. inv K3. inv K2. clear K1.
-                       destruct (Inj_init m1) as [m2 [initMem2 Inj]]; clear Inj_init . apply GenvInit1. apply K5.
-                        assert (X := @Sim_inj.core_initial _ _ _ _ _ _ _ Sem1 Sem2  (Genv.globalenv P1) (Genv.globalenv P2)  entrypoints R _ _ _ Hfound nil _ _ _ nil _ K4 Inj).
-                        (*would need relationship between entrypoints and externidents assert (ZZ: (forall (w1 w2 : val) (sigg : signature),  In (w1,w2, sigg) entrypoints -> val_inject j w1 w2)).
-                             intros.  unfold CompilerCorrectness.entries_inject_ok in ext_ok. apply ext_ok in H1.*)
-                        destruct X as [d' [c2 [iniCore2 Match]]].
-                          constructor.
-                          constructor. 
-                          exists d'. exists (c2,m2). simpl in *.
-                          split; auto. exists b2. exists nil.
-                             repeat  split; try constructor.
-                             rewrite <- H0. apply KK2.
-                             assumption.
-                             apply GenvInit2. apply initMem2.
-                         exists jInit. split; auto. 
-           (*finalstate*)
-                 clear GenvInit1 GenvInit2.
-                 simpl. unfold final_state. intros. destruct s1 as [c1 m1]. destruct s2 as [c2 m2]. simpl in *.
-                      destruct H1 as [j [InjJ MCJ]]; simpl in *.
-                      apply (Sim_inj.core_halted R _ _ _ _ _ _ _ MCJ H2).
-           (*diagram*) 
-                 clear GenvInit1 GenvInit2.
-                 simpl. subst fsim_match_states. simpl. intros.
-                destruct s1 as [c1 m1]. destruct s2 as [c2 m2].  destruct s1' as [c1' m1'].  simpl in *.
-                destruct H2 as [j [InjJ MCJ]].
-                 inv H1. 
-                 (*corestep*)  
-                   assert (DD := @Sim_inj.core_diagram _ _ _ _ _ _ _ Sem1 Sem2 (Genv.globalenv P1) (Genv.globalenv P2) entrypoints R _ _ _ _ H5 _ _ _ _ MCJ).
-                   destruct DD as [c2' [m2' [d' [j' [InjJ' [Sep [MC' myStep]]]]]]].
-                  exists d'. exists (c2', m2'); simpl. split; auto.
-                    destruct myStep.
-                      (*case corestep_plus*) left. eapply corestep_plus_plus_step; eauto.
-                      (*case core_step_star*) right.  destruct H1. split; auto. apply corestep_star_star_step; eauto.
-                   exists j'; split; auto. eapply inject_incr_trans. apply InjJ. apply InjJ'.                    
-               (*external_step*) 
-                    destruct (@Sim_inj.core_at_external _ _ _ _ _ _ _ Sem1 Sem2 (Genv.globalenv P1) (Genv.globalenv P2) entrypoints R _ _ _ _ _ _ _ _ MCJ H7) 
-                               as[INJ [jPG [args2 [LD [TP AtExt2]]]]].
-                    (*LENB: HERE's where we need that j preserves globals.
-                            assert (HH: meminj_preserves_globals (Genv.globalenv P1) j).
-                       eapply meminj_preserves_globals_inject_incr. apply preserves_globals. apply InjJ.*)
-                           (* it seems inject doesn't preserve globals!
-                             split; intros. destruct HGenv1. apply (H3 _ (id, CompilerCorrectness.extern_func (ef_sig ef))) in H8.  apply ext_ok in H8.
-                                    destruct H8 as [b1 [b2 [Hb1 [Hb2 [Hb1b2 _]]]]]. rewrite Hb1 in H1. inv H1.  apply InjJ. assumption.*)
-                    apply forall_inject_val_list_inject in LD.
-                    assert (ZZ:= @external_call_mem_inject ef  _ _ (Genv.globalenv P1) _ _ _ _ _ j _ _ jPG H8 INJ LD).
-                    destruct ZZ as [j'  [ret2 [m2' [extCall2 [RetInj [MInj2 [Munch1 [Munch2 [InjJ' Sep']]]]]]]]].
-                    assert (extCall2Genv2 : external_call ef (Genv.globalenv P2) args2 m2 t ret2 m2'). 
-                         eapply external_call_symbols_preserved_gen. 
-                             apply HypGenv. (*HERE*) 
-                             apply HypVolatile. (*HERE*)
-                             apply extCall2.
-                          (*An alternative would be the following proof of extCall2Genv2:
-                                    apply (@external_call_symbols_preserved_2 ef F1 V1 F2 V2 (fun v1 =>Errors.Error nil)) with (ge1:=(Genv.globalenv P1)).
-                                          apply extCall2.
-                                          admit. (*symmetric hypothesis on Genv.findSymbol*) 
-                                          simpl. admit. (*first hyp on globvars*) 
-                                          simpl. admit. (*second hyp on globvars*) *)
-                    clear extCall2.
-                    assert (DD := @Sim_inj.core_after_external _ _ _ _ _ _ _ Sem1 Sem2 (Genv.globalenv P1) (Genv.globalenv P2) 
-                                               entrypoints R i j).
-                    assert (RetTp:= external_call_well_typed _ _ _ _ _ _ _ H8).
-                    destruct (DD j' _ _ _ _ _ _ _ _ _ _ INJ MCJ H7 jPG InjJ' Sep' MInj2 RetInj) as [d' [c1'' [c2' [AftExt1 [AftExt2 Match2]]]]]; clear DD.
-                         eapply external_call_mem_forward; eauto.
-                         apply Munch1.
-                         eapply external_call_mem_forward; eauto.
-                         apply Munch2.
-                         eapply external_call_well_typed. apply extCall2Genv2. 
-                      rewrite AftExt1 in H9. inv H9.
-                         exists d'. exists (c2', m2').
-                         split. left. apply plus_one. eapply  step_ext_step. apply AtExt2. apply extCall2Genv2. apply AftExt2. 
-                         exists j'; simpl.  split;eauto. eapply inject_incr_trans. apply InjJ. apply InjJ'.
-         (* fsim_symbols_preserved*) simpl. apply HypGenv. (*SAME HERE*)
-Qed.
-(*
-1. The need for the axiom GenvHyp in all cases (or alternatively the addition of axioms  HypGenv and HypVolatile, 
-     at the beginning of all cases): 
-These are needed in order to apply external_call_symbols_preserved_gen, in order to establish external_call 
-ef (GEnv P2) vargs m1 t vres m2, 
-As mentioned in the file, an alternative proof of this fact using external_call_symbols_preserved_2 would require 
-a slightly different axiom on globvars, eliminating the need for HypVolatile.
-Additionally, HypGenv is also explicitly required in order to discharge Xavier's condition  fsim_symbols_preserved.
-
-2. The need to establish a "meminj_preserves_globals" property in case inject-diamond-externalStep.
-I temporarily added the condition meminj_preserves_globals jInit in cc_inj, with the idea
-  that we would thread it through the execution. But meminj_preserves_globals is formally 
-  not preserved by inj_incr. But maybe the 3rd clause in meminj_preserves_globals is
-  stronger than what's needed to prove the CompCert phases?
-
-An alternative (maybe this is needed in any case) would be to have at_external
-   (or maybe external_call ef ge vargs m1 t vres m2 in general)  
-  imply that (f,d) in ExternIdent, so that we can apply entries_ok or entries_inject_ok.
-  But: some externals_funstions ("builtins") dont have idents - so maybe ExternIdents should be
-        of a different type, not take idents? Or maybe should differentiate in external_description
-         between builtins and nonbuiltins?
-
-It seems given the strong condition imposed by meminj_preserves_global, our choice to
-differentiate between entries_ok and entries_inject_ok is too fine for current CompCert.
-Maybe we soulh use entries_ok even in inject-case (at least for the sake of demonstrating 
-that our approach works)?
-
-3. Do we still need the allowed_modifications stuff??
- *)
-
-End COMPILER_CORRECTNESS_COMPCERT_SIM.
-(*
-meminj_preserves_globals:
-  - defined in Events (so quite at a high level)
-  - established ONLY in cfrontend/Cminorgenproof (no other compiler phase establishes it!) via the
-    following lemma:
-      Remark inj_preserves_globals: forall f hi, match_globalenvs f hi -> meminj_preserves_globals ge f.
-*)
     
